code/ecdsap256/Hacl.Impl.P256.Signature.Common.fst
@@ -300,7 +300,7 @@ val multByOrder2: #c: curve -> result: point c ->  p: point c -> tempBuffer: lbu
   )
   (ensures fun h0 _ h1  -> modifies (loc result |+| loc tempBuffer) h0 h1 /\
     (
-      let xN, yN, zN = scalar_multiplication (prime_order_seq #P256) (point_prime_to_coordinates c (as_seq h0 p)) in 
+      let xN, yN, zN = scalar_multiplication #c (prime_order_seq #P256) (point_prime_to_coordinates c (as_seq h0 p)) in 
       let x3, y3, z3 = point_x_as_nat c h1 result, point_y_as_nat c h1 result, point_z_as_nat c h1 result in 
       x3 == xN /\ y3 == yN /\ z3 == zN 
     )
@@ -329,7 +329,7 @@ val isOrderCorrect: #c: curve -> p: point c -> tempBuffer: lbuffer uint64 (size 
   )
   (ensures fun h0 r h1 -> 
     modifies(loc tempBuffer) h0 h1 /\ 
-    (let (xN, yN, zN) = scalar_multiplication (prime_order_seq #P256) (point_prime_to_coordinates c (as_seq h0 p)) in 
+    (let (xN, yN, zN) = scalar_multiplication #c (prime_order_seq #P256) (point_prime_to_coordinates c (as_seq h0 p)) in 
      r == Spec.P256.isPointAtInfinity (xN, yN, zN))
   )
 
