code/ecdsap256/Hacl.Spec.P256.MontgomeryMultiplication.fst
@@ -13,81 +13,107 @@ open Lib.IntTypes
 
 #set-options "--z3rlimit 40 --fuel 0 --ifuel 0"
 
-let fromDomain_ #c a = (a * modp_inv2 #c (pow2 (getPower c))) % (getPrime c)
 
+let fromDomain_ #c a = a * modp_inv2 #c (pow2 (getPower c)) % (getPrime c)
 
 let fromDomainPoint #c a =
   let x, y, z = a in
   fromDomain_ #c x, fromDomain_ #c y, fromDomain_ #c z
 
 
-let toDomain_ #c a = (a * pow2 (getPower c)) % (getPrime c)
-
+let toDomain_ #c a = a * pow2 (getPower c) % (getPrime c)
 
 let lemmaFromDomain a = ()
 
-
-let lemmaToDomain a = ()
+let lemmaToDomain #c a = ()
 
 
 let lemmaToDomainAndBackIsTheSame #c a =
-  admit();
+  let power = getPower2 c in 
+  let prime = getPrime c in 
+  
   let to = toDomain_ #c a in
   lemmaToDomain #c a;
   let from = fromDomain_ #c to in
   lemmaFromDomain #c to;
-  lemma_mod_mul_distr_l (a * pow2 256) (modp_inv2 #P256 (pow2 256)) prime256;
+  lemma_mod_mul_distr_l (a * power) (modp_inv2 #c power) prime;
+  
   assert_norm (pow2 256 * modp_inv2 #P256 (pow2 256) % prime256 = 1);
-  modulo_distributivity_mult_last_two a 1 1 (pow2 256) (modp_inv2 #P256 (pow2 256)) prime256;
-  modulo_lemma a (getPrime c)
+  assert_norm (pow2 384 * modp_inv2 #P384 (pow2 384) % prime384 = 1);
+  
+  modulo_distributivity_mult_last_two a 1 1 power (modp_inv2 #c power) prime;
+  modulo_lemma a prime
 
 
 let lemmaFromDomainToDomain #c a =
   let prime = getPrime c in 
+  let power = getPower2 c in 
+  
   let from = fromDomain_ #c a in
   lemmaFromDomain #c a;
   let to = toDomain_ #c from in
   lemmaToDomain #c from;
-  lemma_mod_mul_distr_l (a * modp_inv2 #P256 (pow2 256)) (pow2 256)  prime256;
-  assert_norm (modp_inv2 #P256 (pow2 256) * (pow2 256) % prime = 1);
-  modulo_distributivity_mult_last_two a 1 1 (modp_inv2 #P256 (pow2 256)) (pow2 256) prime256;
+  lemma_mod_mul_distr_l (a * modp_inv2 #c power) power prime;
+  
+  assert_norm (modp_inv2 #P256 (pow2 256) * (pow2 256) % prime256 = 1);
+  assert_norm (modp_inv2 #P384 (pow2 384) * (pow2 384) % prime384 = 1);
+  
+  modulo_distributivity_mult_last_two a 1 1 (modp_inv2 #c power) power prime;
   modulo_lemma a prime
 
 
-let lemmaFromDomainToDomainModuloPrime a =
-  lemma_mod_mul_distr_l (a*pow2 256) (modp_inv2 #P256 (pow2 256)) prime256;
+let lemmaFromDomainToDomainModuloPrime #c a =
+  let prime = getPrime c in 
+  let power = getPower2 c in 
+  
+  lemma_mod_mul_distr_l (a * power) (modp_inv2 #c power) prime;
+  
   assert_norm (pow2 256 * modp_inv2 #P256 (pow2 256) % prime256 = 1);
-  modulo_distributivity_mult_last_two a 1 1 (pow2 256) (modp_inv2 #P256 (pow2 256)) prime256
+  assert_norm (pow2 384 * modp_inv2 #P384 (pow2 384) % prime384 = 1);
+  
+  modulo_distributivity_mult_last_two a 1 1 power (modp_inv2 #c power) prime
 
 
-let inDomain_mod_is_not_mod a =
-  lemma_mod_mul_distr_l a (pow2 256) prime256
+let inDomain_mod_is_not_mod #c a =
+  let prime = getPrime c in 
+  let power = getPower2 c in 
+
+  lemma_mod_mul_distr_l a power prime
 
 
 let multiplicationInDomainNat #c #k #l a b =
   let prime = getPrime c in 
-  assert_norm (prime256 > 3);
-  let multResult = a * b * modp_inv2_prime (pow2 256) prime256 % prime256 in
-  modulo_distributivity_mult2 (k * pow2 256) (l * pow2 256) (modp_inv2_prime (pow2 256) prime256) prime;
-  lemma_twice_brackets k (pow2 256) 1 l (pow2 256) 1 (modp_inv2 #P256 (pow2 256));
-  assert_norm (pow2 256 * modp_inv2 #P256 (pow2 256) % prime == 1);
-  modulo_distributivity_mult_last_two k (pow2 256) l (pow2 256) (modp_inv2 #P256 (pow2 256)) prime;
-  lemma_mul_associativity_3 k (pow2 256) l
+  let power = getPower2 c in 
+
+  let multResult = a * b * modp_inv2_prime power prime % prime in
+  
+  modulo_distributivity_mult2 (k * power) (l * power) (modp_inv2_prime power prime) prime;
+  lemma_twice_brackets k power 1 l power 1 (modp_inv2 #c power);
+  
+  assert_norm (pow2 256 * modp_inv2 #P256 (pow2 256) % prime256 == 1);
+  assert_norm (pow2 384 * modp_inv2 #P384 (pow2 384) % prime384 == 1);
+    
+  modulo_distributivity_mult_last_two k power l power (modp_inv2 #c power) prime;
+  lemma_mul_associativity_3 k power l
+
 
 let additionInDomain #c a b =
   let prime = getPrime c in 
+  let power = getPower2 c in 
+  
   let k = fromDomain_ #c a in
   let l = fromDomain_ #c b in
+  
   calc (==) {
-    (a + b) % prime256;
+    (a + b) % prime;
     == { lemmaFromDomainToDomain #c a; lemmaFromDomainToDomain #c b }
-    (toDomain_ #c k + toDomain_ #c l) % prime256;
+    (toDomain_ #c k + toDomain_ #c l) % prime;
     == { }
-    (k * pow2 256 % prime256 + l * pow2 256 % prime256) % prime256;
-    == { modulo_distributivity (k * pow2 256) (l * pow2 256) prime }
-    (k * pow2 256 + l * pow2 256) % prime256;
-    == { distributivity_add_left k l (pow2 256) }
-    ((k + l) * pow2 256) % prime256;
+    (k * power % prime + l * power % prime) % prime;
+    == { modulo_distributivity (k * power) (l * power) prime }
+    (k * power + l * power) % prime;
+    == { distributivity_add_left k l power }
+    ((k + l) * power) % prime;
     == { }
     toDomain_ #c (fromDomain_ #c a + fromDomain_ #c b);
   }
@@ -95,38 +121,45 @@ let additionInDomain #c a b =
 
 let substractionInDomain #c a b =
   let prime = getPrime c in 
+  let power = getPower2 c in 
+  
   let k = fromDomain_ #c a in
   let l = fromDomain_ #c b in
+  
   calc (==) {
-    (a - b) % prime256;
+    (a - b) % prime;
     == { lemmaFromDomainToDomain #c a; lemmaFromDomainToDomain #c b }
-    (toDomain_ #c k - toDomain_ #c l) % prime256;
+    (toDomain_ #c k - toDomain_ #c l) % prime;
     == { }
-    (k * pow2 256 % prime256 - l * pow2 256 % prime256) % prime256;
-    == { lemma_mod_sub_distr (k * pow2 256 % prime256) (l * pow2 256) prime }
-    (k * pow2 256 % prime256 - l * pow2 256) % prime256;
-    == { lemma_mod_add_distr (-(l * pow2 256)) (k * pow2 256) prime }
-    (k * pow2 256 - l * pow2 256) % prime256;
-    == { distributivity_sub_left k l (pow2 256) }
-    ((k - l) * pow2 256) % prime256;
+    (k * power % prime - l * power % prime) % prime;
+    == { lemma_mod_sub_distr (k * power % prime) (l * power) prime }
+    (k * power % prime - l * power) % prime;
+    == { lemma_mod_add_distr (-(l * power)) (k * power) prime }
+    (k * power - l * power) % prime;
+    == { distributivity_sub_left k l power }
+    ((k - l) * power) % prime;
     == { }
     toDomain_ #c (fromDomain_ #c a - fromDomain_ #c b);
   }
 
+
 open Lib.ByteSequence
 
-val ith_bit_power: k:lbytes 32 -> i:nat{i < 256}
+val ith_bit_power: #c: curve -> k:lbytes (getCoordinateLen c) 
+  -> i:nat{i < (getCoordinateLen c) * 8}
   -> t:uint64 {(v t == 0 \/ v t == 1) /\ v t == nat_from_intseq_le k / pow2 i % 2}
 
-let ith_bit_power k i =
+let ith_bit_power #c k i =
   let q = i / 8 in
   let r = i % 8 in
   let tmp1 = k.[q] >>. (size r) in
   let tmp2 = tmp1 &. u8 1 in
   let res = to_u64 tmp2 in
+  
   logand_le tmp1 (u8 1);
   logand_mask tmp1 (u8 1) 1;
-  lemma_scalar_ith P256 k q;
+  lemma_scalar_ith c k q;
+  
   let k = nat_from_intseq_le k in
   pow2_modulo_division_lemma_1 (k / pow2 (8 * (i / 8))) (i % 8) 8;
   division_multiplication_lemma k (pow2 (8 * (i / 8))) (pow2 (i % 8));
@@ -154,39 +187,44 @@ let lemma_swaped_steps p q = ()
 
 open Lib.ByteSequence
 
-let _pow_step k i (p, q) =
-  let bit = 255 - i in
-  let bit = ith_bit_power k bit in
+let _pow_step #c k i (p, q) =
+  let bit = (getCoordinateLen c) * 8 -1 - i in
+  let bit = ith_bit_power #c k bit in
   let open Lib.RawIntTypes in
   if uint_to_nat bit = 0 then _pow_step0 p q else _pow_step1 p q
 
 
-
-val lemma_even: index:pos{index <= 256} -> k:lseq uint8 32 {v (ith_bit_power k (256 - index)) == 0} ->
+val lemma_even: #c: curve 
+  -> index:pos{index <= (getCoordinateLen c) * 8} 
+  -> k:lseq uint8 (getCoordinateLen c) 
+    {v (ith_bit_power k ((getCoordinateLen c) * 8 - index)) == 0} ->
   Lemma (
     let number = nat_from_bytes_le k in
-    let newIndex = 256 - index in
+    let newIndex = (getCoordinateLen c) * 8 - index in
     2 * arithmetic_shift_right number (newIndex + 1) ==
     arithmetic_shift_right number newIndex)
 
-let lemma_even index k =
+let lemma_even #c index k =
   let number = nat_from_bytes_le k in
-  let n = 256 - index in
+  let n = (getCoordinateLen c) * 8 - index in
   FStar.Math.Lemmas.pow2_double_mult n;
   lemma_div_def (number / pow2 n) 2;
   FStar.Math.Lemmas.division_multiplication_lemma number (pow2 n) 2
 
 
-val lemma_odd: index:pos{index <= 256} -> k:lseq uint8 32 {uint_v (ith_bit_power k (256 - index)) == 1} ->
+val lemma_odd: #c: curve 
+  -> index:pos{index <= (getCoordinateLen c) * 8} 
+  -> k:lseq uint8 (getCoordinateLen c) 
+    {uint_v (ith_bit_power k ((getCoordinateLen c) * 8 - index)) == 1} ->
   Lemma(
     let number = nat_from_intseq_le k in
-    let n = 256 - index  in
+    let n = (getCoordinateLen c) * 8 - index  in
     2 * arithmetic_shift_right number (n + 1) + 1 ==
     arithmetic_shift_right number n)
 
-let lemma_odd index k =
+let lemma_odd #c index k =
   let number = nat_from_bytes_le k in
-  let n = 256 - index in
+  let n = (getCoordinateLen c) * 8 - index in
   let a0 = 2 * arithmetic_shift_right number (n + 1) + 1 in
   lemma_div_def (number / pow2 n) 2;
   division_multiplication_lemma number (pow2 n) 2;
@@ -217,107 +255,115 @@ val lemma_exponen_spec_0:
   -> k: scalar_bytes #c
   -> start:tuple2 nat_prime nat_prime {let st0, _ = start in st0 == 1} 
   -> Lemma (
+    let prime = getPrime c in 
     let start0, start1 = start in
     let number = nat_from_bytes_le k in
-    let newIndex = 256 in
+    let newIndex = (getCoordinateLen c) * 8 in
     let f0, f1 = Lib.LoopCombinators.repeati 0 (_pow_step #c k) start in
-    f0 == pow start1 (arithmetic_shift_right number newIndex) % prime256 /\
-    f1 == pow start1 (arithmetic_shift_right number newIndex + 1) % prime256
+    f0 == pow start1 (arithmetic_shift_right number newIndex) % prime /\
+    f1 == pow start1 (arithmetic_shift_right number newIndex + 1) % prime
   )
 
-let lemma_exponen_spec_0 k start =
+let lemma_exponen_spec_0 #c k start =
+  let prime = getPrime c in 
+  let power = getPower2 c in 
+
   let st0, st1 = start in
   let number = nat_from_bytes_le #SEC k in
-    assert (arithmetic_shift_right number 256 == number / pow2 256);
-  FStar.Math.Lemmas.lemma_div_lt_nat number 256 256;
-    assert (arithmetic_shift_right number 256 == 0);
-  Lib.LoopCombinators.eq_repeati0 256 (_pow_step k) start;
-  FStar.Math.Lemmas.small_modulo_lemma_1 st1 prime256
+    assert (arithmetic_shift_right number (getPower c) == number / power);
+  FStar.Math.Lemmas.lemma_div_lt_nat number (getPower c) (getPower c);
+    assert (arithmetic_shift_right number (getPower c) == 0);
+  Lib.LoopCombinators.eq_repeati0 (getPower c) (_pow_step k) start;
+  FStar.Math.Lemmas.small_modulo_lemma_1 st1 prime
 
 
 #pop-options
 
-let rec lemma_exponen_spec k start index =
+let rec lemma_exponen_spec #c k start index =
+  let prime = getPrime c in 
+  let power = getPower2 c in 
+
   let f = _pow_step k in
   let st0, st1 = start in
   let number = nat_from_bytes_le k in
-  let newIndex = 256 - index in
+  let newIndex = (getCoordinateLen c) * 8 - index in
   let open Lib.LoopCombinators in
   match index with
   | 0 -> lemma_exponen_spec_0 k start
   | _ ->
     begin
-    unfold_repeati 256 f start (index - 1);
+    let p2 = getPower c in 
+    unfold_repeati p2 f start (index - 1);
     lemma_exponen_spec k start (index - 1);
-    let bitMask = uint_v (ith_bit_power k (256 - index)) in
+    let bitMask = uint_v (ith_bit_power #c k (p2 - index)) in
     match bitMask with
       | 0 ->
-        let a0 = pow st1 (arithmetic_shift_right number (256 - index + 1)) in
-        let a1 = pow st1 (arithmetic_shift_right number (256 - index + 1) + 1) in
+        let a0 = pow st1 (arithmetic_shift_right number (p2 - index + 1)) in
+        let a1 = pow st1 (arithmetic_shift_right number (p2 - index + 1) + 1) in
         calc (==) {
-          (a0 % prime256) * (a0 % prime256) % prime256;
-          == {modulo_distributivity_mult a0 a0 prime256}
-          (a0 * a0) % prime256;
+          (a0 % prime) * (a0 % prime) % prime;
+          == {modulo_distributivity_mult a0 a0 prime}
+          (a0 * a0) % prime;
           == { }
-          (pow st1 (arithmetic_shift_right number (256 - index + 1)) * pow st1 (arithmetic_shift_right number (256 - index + 1))) % prime256;
-          == {pow_plus st1 (arithmetic_shift_right number (256 - index + 1)) (arithmetic_shift_right number (256 - index + 1))}
-          (pow st1 (arithmetic_shift_right number (256 - index + 1) + arithmetic_shift_right number (256 - index + 1))) % prime256;
+          (pow st1 (arithmetic_shift_right number (p2 - index + 1)) * pow st1 (arithmetic_shift_right number (p2 - index + 1))) % prime;
+          == {pow_plus st1 (arithmetic_shift_right number (p2 - index + 1)) (arithmetic_shift_right number (p2 - index + 1))}
+          (pow st1 (arithmetic_shift_right number (p2 - index + 1) + arithmetic_shift_right number (p2 - index + 1))) % prime;
           == {}
-          (pow st1 (2 * arithmetic_shift_right number (256 - index + 1))) % prime256;
-          == {lemma_even index k}
-          pow st1 (arithmetic_shift_right number newIndex) % prime256;
+          (pow st1 (2 * arithmetic_shift_right number (p2 - index + 1))) % prime;
+          == {lemma_even #c index k}
+          pow st1 (arithmetic_shift_right number newIndex) % prime;
         };
         calc (==) {
-          (a0 % prime256) * (a1 % prime256) % prime256;
-          == {modulo_distributivity_mult a0 a1 prime256}
-          (a0 * a1) % prime256;
+          (a0 % prime) * (a1 % prime) % prime;
+          == {modulo_distributivity_mult a0 a1 prime}
+          (a0 * a1) % prime;
           == { }
-          (pow st1 (arithmetic_shift_right number (256 - index + 1)) * pow st1 (arithmetic_shift_right number (256 - index + 1) + 1)) % prime256;
-          == {pow_plus st1 (arithmetic_shift_right number (256 - index + 1)) (arithmetic_shift_right number (256 - index + 1) + 1)}
-          (pow st1 (arithmetic_shift_right number (256 - index + 1) + arithmetic_shift_right number (256 - index + 1) + 1)) % prime256;
+          (pow st1 (arithmetic_shift_right number (p2 - index + 1)) * pow st1 (arithmetic_shift_right number (p2 - index + 1) + 1)) % prime;
+          == {pow_plus st1 (arithmetic_shift_right number (p2 - index + 1)) (arithmetic_shift_right number (p2 - index + 1) + 1)}
+          (pow st1 (arithmetic_shift_right number (p2 - index + 1) + arithmetic_shift_right number (p2 - index + 1) + 1)) % prime;
           == {}
-          (pow st1 (2* arithmetic_shift_right number (256 - index + 1) + 1)) % prime256;
-          == {lemma_even index k}
-          (pow st1 (arithmetic_shift_right number (256 - index) + 1)) % prime256;
+          (pow st1 (2 * arithmetic_shift_right number (p2 - index + 1) + 1)) % prime;
+          == {lemma_even #c index k}
+          (pow st1 (arithmetic_shift_right number (p2 - index) + 1)) % prime;
         }
       | 1 ->
-        let a0 = pow st1 (arithmetic_shift_right number (256 - index + 1)) in
-        let a1 = pow st1 (arithmetic_shift_right number (256 - index + 1) + 1) in
+        let a0 = pow st1 (arithmetic_shift_right number (p2 - index + 1)) in
+        let a1 = pow st1 (arithmetic_shift_right number (p2 - index + 1) + 1) in
         calc (==) {
-          (a1 % prime256) * (a1 % prime256) % prime256;
-          == {modulo_distributivity_mult a1 a1 prime256}
-          (a1 * a1) % prime256;
+          (a1 % prime) * (a1 % prime) % prime;
+          == {modulo_distributivity_mult a1 a1 prime}
+          (a1 * a1) % prime;
           == { }
-          (pow st1 (arithmetic_shift_right number (256 - index + 1) + 1) * pow st1 (arithmetic_shift_right number (256 - index + 1) + 1)) % prime256;
-          == {pow_plus st1 (arithmetic_shift_right number (256 - index + 1) + 1) (arithmetic_shift_right number (256 - index + 1) + 1)}
-          (pow st1 (arithmetic_shift_right number (256 - index + 1) + 1 + arithmetic_shift_right number (256 - index + 1) + 1)) % prime256;
+          (pow st1 (arithmetic_shift_right number (p2 - index + 1) + 1) * pow st1 (arithmetic_shift_right number (p2 - index + 1) + 1)) % prime;
+          == {pow_plus st1 (arithmetic_shift_right number (p2 - index + 1) + 1) (arithmetic_shift_right number (p2 - index + 1) + 1)}
+          (pow st1 (arithmetic_shift_right number (p2 - index + 1) + 1 + arithmetic_shift_right number (p2 - index + 1) + 1)) % prime;
           == {}
-          (pow st1 (2 * arithmetic_shift_right number (256 - index + 1) + 2)) % prime256;
-          == {lemma_odd index k}
-          pow st1 (arithmetic_shift_right number newIndex + 1) % prime256;
+          (pow st1 (2 * arithmetic_shift_right number (p2 - index + 1) + 2)) % prime;
+          == {lemma_odd #c index k}
+          pow st1 (arithmetic_shift_right number newIndex + 1) % prime;
         };
         calc (==) {
-          (a0 % prime256) * (a1 % prime256) % prime256;
-          == {modulo_distributivity_mult a0 a1 prime256}
-          (a0 * a1) % prime256;
+          (a0 % prime) * (a1 % prime) % prime;
+          == {modulo_distributivity_mult a0 a1 prime}
+          (a0 * a1) % prime;
           == { }
-          (pow st1 (arithmetic_shift_right number (256 - index + 1)) * pow st1 (arithmetic_shift_right number (256 - index + 1) + 1)) % prime256;
-          == {pow_plus st1 (arithmetic_shift_right number (256 - index + 1)) (arithmetic_shift_right number (256 - index + 1) + 1)}
-          (pow st1 (arithmetic_shift_right number (256 - index + 1) + arithmetic_shift_right number (256 - index + 1) + 1)) % prime256;
+          (pow st1 (arithmetic_shift_right number (p2 - index + 1)) * pow st1 (arithmetic_shift_right number (p2 - index + 1) + 1)) % prime;
+          == {pow_plus st1 (arithmetic_shift_right number (p2 - index + 1)) (arithmetic_shift_right number (p2 - index + 1) + 1)}
+          (pow st1 (arithmetic_shift_right number (p2 - index + 1) + arithmetic_shift_right number (p2 - index + 1) + 1)) % prime;
           == {}
-          (pow st1 (2* arithmetic_shift_right number (256 - index + 1) + 1)) % prime256;
-          == {lemma_odd index k}
-          (pow st1 (arithmetic_shift_right (nat_from_bytes_le k) (256 - index)) % prime256);
+          (pow st1 (2 * arithmetic_shift_right number (p2 - index + 1) + 1)) % prime;
+          == {lemma_odd #c index k}
+          (pow st1 (arithmetic_shift_right (nat_from_bytes_le k) (p2 - index)) % prime);
         }
     end
 
 
-let pow_spec k p =
-  assert_norm (1 < prime256);
-  let a, b = Lib.LoopCombinators.repeati 256 (_pow_step k) (1, p) in 
-  lemma_exponen_spec k (1, p) 256;
+let pow_spec #c k p =
+  let a, b = Lib.LoopCombinators.repeati (getPower c) (_pow_step k) (1, p) in 
+  lemma_exponen_spec k (1, p) (getPower c);
   a
 
 
-let sq_root_spec a = 
-  pow a ((prime256 + 1) / 4) % prime256
+let sq_root_spec #c a = 
+  let prime = getPrime c in 
+  pow a ((prime + 1) / 4) % prime
