specs/ecdsap256/Spec.ECDSA.fst
@@ -1,3 +1,4 @@
+
 module Spec.ECDSA
 
 open FStar.Mul
@@ -18,10 +19,10 @@ open FStar.Math.Lib
 
 #set-options "--z3rlimit 200"
 
-val ith_bit: #c: curve -> k:lbytes (getCoordinateLen c) -> i:nat{i < getPower c}
+val ith_bit_felem: #c: curve -> k:lbytes (getCoordinateLen c) -> i:nat{i < getPower c}
   -> t:uint64 {(v t == 0 \/ v t == 1) /\ v t == nat_from_intseq_le k / pow2 i % 2}
 
-let ith_bit #c k i =
+let ith_bit_felem #c k i =
   let q = i / 8 in
   let r = i % 8 in
   let tmp1 = k.[q] >>. (size r) in
@@ -85,7 +86,7 @@ val _exp_step: #c: curve
 
 let _exp_step #c k i (p, q) =
   let bit = (getPower c - 1) - i in
-  let bit = ith_bit k bit in
+  let bit = ith_bit_felem k bit in
   let open Lib.RawIntTypes in
   if uint_to_nat bit = 0 then _exp_step0 p q else _exp_step1 p q
 
@@ -102,7 +103,7 @@ let _exponent_spec #c k (p, q) =
 
 val lemma_even: #c: curve 
   -> index:pos{index <= getPower c} 
-  -> k:lseq uint8 (getCoordinateLen c) {v (ith_bit k (getPower c - index)) == 0} ->
+  -> k:lseq uint8 (getCoordinateLen c) {v (ith_bit_felem k (getPower c - index)) == 0} ->
   Lemma (
     let number = nat_from_bytes_le k in
     let newIndex = (getPower c) - index in
@@ -117,7 +118,7 @@ let lemma_even #c index k =
   FStar.Math.Lemmas.division_multiplication_lemma number (pow2 n) 2
 
 
-val lemma_odd: #c: curve -> index:pos{index <= getPower c} -> k:lseq uint8 (getCoordinateLen c) {uint_v (ith_bit k (getPower c - index)) == 1} ->
+val lemma_odd: #c: curve -> index:pos{index <= getPower c} -> k:lseq uint8 (getCoordinateLen c) {uint_v (ith_bit_felem k (getPower c - index)) == 1} ->
   Lemma(
     let number = nat_from_intseq_le k in 
     let n = getPower c - index  in
@@ -187,7 +188,7 @@ let rec lemma_exponen_spec #c k start index =
     begin
     unfold_repeati (getPower c) f start (index - 1);
     lemma_exponen_spec k start (index - 1);
-    let bitMask = uint_v (ith_bit k ((getPower c) - index)) in
+    let bitMask = uint_v (ith_bit_felem k ((getPower c) - index)) in
     match bitMask with
       | 0 ->
         let a0 = pow st1 (arithmetic_shift_right number (power - index + 1)) in
@@ -329,7 +330,7 @@ let verifyQValidCurvePointSpec #c publicKey =
   y < prime &&
   z < prime &&
   isPointOnCurve #c (x, y, z) &&
-  isPointAtInfinity (scalar_multiplication (prime_order_seq #c) publicKey)
+  isPointAtInfinity (scalar_multiplication #c (prime_order_seq #c) publicKey)
 
 
 val checkCoordinates: #c: curve ->  r: nat -> s: nat -> bool
@@ -450,7 +451,7 @@ let ecdsa_signature_agile c alg mLen m privateKey k =
   assert_norm (pow2 32 < pow2 61);
   assert_norm (pow2 32 < pow2 125);
   let order = getOrder #c in 
-  let r, _ = montgomery_ladder_spec k ((0,0,0), basePoint) in
+  let r, _ = montgomery_ladder_spec k ((0,0,0), (basePoint #c)) in
   let (xN, _, _) = _norm r in
   let hashM = hashSpec c alg mLen m in 
   let z = nat_from_bytes_be hashM % order in
